examples/low-level/crypto/Crypto.Symmetric.PRF.fst
@@ -73,7 +73,7 @@ let above #i x z = x.iv = z.iv && x.ctr >=^ z.ctr
 // the range of our PRF, after idealization and "reverse inlining."
 // for one-time-pads, we keep both the plain and cipher blocks, instead of their XOR.
 
-type smac (rgn:region) (i:id) x = mac: CMA.state (i,x.iv) { CMA.State.region mac = rgn }
+type smac (rgn:region) (i:id) x = mac: CMA.state (i,x.iv) { CMA.State?.region mac = rgn }
 noeq type otp (i:id) = | OTP: l:u32 {l <=^ blocklen i} -> plain i (v l) -> cipher:lbytes (v l) -> otp i
 
 let ctr_0 (i:id) = if CMA.skeyed i then 1ul else 0ul
@@ -140,7 +140,7 @@ noeq type state (i:id) =
 	   #mac_rgn: region{mac_rgn `HH.extends` rgn} ->
            // key is immutable once generated, we should make it private
            key: lbuffer (v (statelen i)) 
-             {Buffer.frameOf key = rgn /\ ~(HS.MkRef.mm (Buffer.content key))} ->
+             {Buffer.frameOf key = rgn /\ ~(HS.MkRef?.mm (Buffer.content key))} ->
            table: table_t rgn mac_rgn i ->
            state i
 
@@ -231,9 +231,9 @@ val prf_mac:
        | Some mac' -> 
 	 h0 == h1 /\ // when decrypting
 	 mac == mac' /\ 
-	 CMA (MAC.norm h1 mac.r) /\
-	 CMA (Buffer.live h1 mac.s) /\
-	 CMA (mac_log ==> m_contains (ilog mac.log) h1)
+	 CMA.(MAC.norm h1 mac'.r) /\ (* mac shadowed by CMA.mac *)
+	 CMA.(Buffer.live h1 mac'.s) /\ (* mac shadowed by CMA.mac *)
+	 CMA.(mac_log ==> m_contains (ilog mac'.log) h1) (* mac shadowed by CMA.mac *)
        | None ->  // when encrypting, we get the stateful post of MAC.create             
          (match find_mac (HS.sel h1 r) x with 
           | Some mac' -> 
@@ -266,9 +266,10 @@ let prf_mac i t k_0 x =
     let contents = !r in
     match find_mac contents x with
     | Some mac -> 
-      assume (CMA (MAC.norm h0 mac.r)); //TODO: replace this using monotonicity
-      assume (HS (Buffer (CMA (not ((Buffer.content mac.s).mm))))); //TODO: mark this as not manually managed
-      Buffer.recall (CMA mac.s);
+      let mac0 = mac in (* mac shadowed by CMA.mac *)
+      assume (CMA.(MAC.norm h0 mac0.r)); //TODO: replace this using monotonicity
+      assume (HS.(Buffer.(CMA.(not ((Buffer.content mac0.s).mm))))); //TODO: mark this as not manually managed
+      Buffer.recall (CMA.(mac0.s));
       mac
     | None ->
       let mac = CMA.gen t.mac_rgn macId k_0 in
@@ -328,7 +329,7 @@ let prf_sk0 #i t =
           r := SeqProperties.snoc contents (Entry x sk0);
           sk0 in
       assume (HS.is_eternal_region t.mac_rgn);
-      assume (HS (Buffer (CMA (not ((Buffer.content sk0).mm))))); //TODO: mark this as not manually managed
+      assume (HS.(Buffer.(CMA.(not ((Buffer.content sk0).mm))))); //TODO: mark this as not manually managed
       Buffer.recall sk0;
       assume false; //NS: disovered while triaging this file ... unable to prove that (find_sk0 (HS.sel h1 r) x = Some _)
       sk0
