examples/low-level/crypto/Crypto.Symmetric.Poly1305.Lemmas.fst
@@ -50,7 +50,7 @@ private val mk_mask: nbits:FStar.UInt32.t{FStar.UInt32.v nbits < 64} ->
   Tot (z:U64.t{v z == pow2 (FStar.UInt32.v nbits) - 1})
 let mk_mask nbits =
   Math.Lemmas.pow2_lt_compat 64 (FStar.UInt32.v nbits);
-  U64 ((1uL <<^ nbits) -^ 1uL)
+  U64.((1uL <<^ nbits) -^ 1uL)
 
 
 #set-options "--initial_fuel 0 --max_fuel 0 --z3timeout 5"
@@ -268,8 +268,8 @@ let add_disjoint #z a b n m =
   
 val lemma_disjoint_bounded:
   b0:U64.t -> b1:U64.t -> l:nat -> m:pos{m >= l} -> n:nat{n > m /\ n <= 64} ->
-  Lemma (requires (U64 (v b0 < pow2 m /\ v b1 % pow2 m = 0 /\ v b1 < pow2 n /\ v b0 % pow2 l = 0)))
-        (ensures  (U64 (v (b0 |^ b1) = v b0 + v b1 /\ v b0 + v b1 < pow2 n /\ (v b0 + v b1) % pow2 l = 0)))
+  Lemma (requires (U64.(v b0 < pow2 m /\ v b1 % pow2 m = 0 /\ v b1 < pow2 n /\ v b0 % pow2 l = 0)))
+        (ensures  (U64.(v (b0 |^ b1) = v b0 + v b1 /\ v b0 + v b1 < pow2 n /\ (v b0 + v b1) % pow2 l = 0)))
 let lemma_disjoint_bounded b0 b1 l m n =
   let open FStar.UInt64 in
   logor_disjoint (v b1) (v b0) m;
@@ -945,7 +945,7 @@ val lemma_trunc1305_:
     /\ v b13 = ((U64.v a4)%pow2 8)
     /\ v b14 = (U64.v a4 / pow2 8) % pow2 8
     /\ v b15 = (U64.v a4 / pow2 16) % pow2 8 ))
-        (ensures  (U8 (v (b0) + pow2 8 * v (b1) + pow2 16 * v (b2) + pow2 24 * v (b3)
+        (ensures  (U8.(v (b0) + pow2 8 * v (b1) + pow2 16 * v (b2) + pow2 24 * v (b3)
   + pow2 32 * v (b4) + pow2 40 * v (b5) + pow2 48 * v (b6) + pow2 56 * v (b7)
   + pow2 64 * v (b8) + pow2 72 * v (b9) + pow2 80 * v (b10) + pow2 88 * v (b11)
   + pow2 96 * v (b12) + pow2 104 * v (b13) + pow2 112 * v (b14) + pow2 120 * v (b15))
@@ -1091,7 +1091,7 @@ let lemma_trunc1305 hb b ha a =
 #reset-options "--initial_fuel 0 --max_fuel 0 --z3timeout 10"
 
 val lemma_little_endian_4: h:HyperStack.mem -> b:Buffer.buffer U8.t{live h b /\ length b = 4} ->
-  Lemma (little_endian (as_seq h b) = U8 (v (get h b 0) + pow2 8 * v (get h b 1)+ pow2 16 * v (get h b 2)+ pow2 24 * v (get h b 3)))
+  Lemma (little_endian (as_seq h b) = U8.(v (get h b 0) + pow2 8 * v (get h b 1)+ pow2 16 * v (get h b 2)+ pow2 24 * v (get h b 3)))
 let lemma_little_endian_4 h b =
   let s = as_seq h b in
   lemma_little_endian_from_top s;
@@ -1116,10 +1116,10 @@ val lemma_add_word_1:
   Lemma (requires (
     let a' = sub a 4ul 4ul in let a'' = sub a 8ul 4ul in let a''' = sub a 12ul 4ul in
     let a = sub a 0ul 4ul in
-    v a0 = U8 (v (get ha a 0) + pow2 8 * v (get ha a 1)+ pow2 16 * v (get ha a 2)+ pow2 24 * v (get ha a 3))
-    /\ v a4 = U8 (v (get ha a' 0) + pow2 8 * v (get ha a' 1)+ pow2 16 * v (get ha a' 2)+ pow2 24 * v (get ha a' 3))
-    /\ v a8 = U8 (v (get ha a'' 0) + pow2 8 * v (get ha a'' 1)+ pow2 16 * v (get ha a'' 2)+ pow2 24 * v (get ha a'' 3))
-    /\ v a12 = U8 (v (get ha a''' 0) + pow2 8 * v (get ha a''' 1)+ pow2 16 * v (get ha a''' 2)+ pow2 24 * v (get ha a''' 3))))
+    v a0 = U8.(v (get ha a 0) + pow2 8 * v (get ha a 1)+ pow2 16 * v (get ha a 2)+ pow2 24 * v (get ha a 3))
+    /\ v a4 = U8.(v (get ha a' 0) + pow2 8 * v (get ha a' 1)+ pow2 16 * v (get ha a' 2)+ pow2 24 * v (get ha a' 3))
+    /\ v a8 = U8.(v (get ha a'' 0) + pow2 8 * v (get ha a'' 1)+ pow2 16 * v (get ha a'' 2)+ pow2 24 * v (get ha a'' 3))
+    /\ v a12 = U8.(v (get ha a''' 0) + pow2 8 * v (get ha a''' 1)+ pow2 16 * v (get ha a''' 2)+ pow2 24 * v (get ha a''' 3))))
     (ensures (little_endian (as_seq ha a) = v a0 + pow2 32 * v a4 + pow2 64 * v a8 + pow2 96 * v a12))
 let lemma_add_word_1 ha a a0 a4 a8 a12 =
   lemma_as_seq_sub ha a 0ul  4ul;
@@ -1256,14 +1256,14 @@ val lemma_add_word:
     let a = sub a 0ul 4ul in
     let b' = sub b 4ul 4ul in let b'' = sub b 8ul 4ul in let b''' = sub b 12ul 4ul in
     let b = sub b 0ul 4ul in
-    v a0 = U8 (v (get ha a 0) + pow2 8 * v (get ha a 1)+ pow2 16 * v (get ha a 2)+ pow2 24 * v (get ha a 3))
-    /\ v a4 = U8 (v (get ha a' 0) + pow2 8 * v (get ha a' 1)+ pow2 16 * v (get ha a' 2)+ pow2 24 * v (get ha a' 3))
-    /\ v a8 = U8 (v (get ha a'' 0) + pow2 8 * v (get ha a'' 1)+ pow2 16 * v (get ha a'' 2)+ pow2 24 * v (get ha a'' 3))
-    /\ v a12 = U8 (v (get ha a''' 0) + pow2 8 * v (get ha a''' 1)+ pow2 16 * v (get ha a''' 2)+ pow2 24 * v (get ha a''' 3))
-    /\ v b0 = U8 (v (get hb b 0) + pow2 8 * v (get hb b 1)+ pow2 16 * v (get hb b 2)+ pow2 24 * v (get hb b 3))
-    /\ v b4 = U8 (v (get hb b' 0) + pow2 8 * v (get hb b' 1)+ pow2 16 * v (get hb b' 2)+ pow2 24 * v (get hb b' 3))
-    /\ v b8 = U8 (v (get hb b'' 0) + pow2 8 * v (get hb b'' 1)+ pow2 16 * v (get hb b'' 2)+ pow2 24 * v (get hb b'' 3))
-    /\ v b12 = U8 (v (get hb b''' 0) + pow2 8 * v (get hb b''' 1)+ pow2 16 * v (get hb b''' 2)+ pow2 24 * v (get hb b''' 3))))
+    v a0 = U8.(v (get ha a 0) + pow2 8 * v (get ha a 1)+ pow2 16 * v (get ha a 2)+ pow2 24 * v (get ha a 3))
+    /\ v a4 = U8.(v (get ha a' 0) + pow2 8 * v (get ha a' 1)+ pow2 16 * v (get ha a' 2)+ pow2 24 * v (get ha a' 3))
+    /\ v a8 = U8.(v (get ha a'' 0) + pow2 8 * v (get ha a'' 1)+ pow2 16 * v (get ha a'' 2)+ pow2 24 * v (get ha a'' 3))
+    /\ v a12 = U8.(v (get ha a''' 0) + pow2 8 * v (get ha a''' 1)+ pow2 16 * v (get ha a''' 2)+ pow2 24 * v (get ha a''' 3))
+    /\ v b0 = U8.(v (get hb b 0) + pow2 8 * v (get hb b 1)+ pow2 16 * v (get hb b 2)+ pow2 24 * v (get hb b 3))
+    /\ v b4 = U8.(v (get hb b' 0) + pow2 8 * v (get hb b' 1)+ pow2 16 * v (get hb b' 2)+ pow2 24 * v (get hb b' 3))
+    /\ v b8 = U8.(v (get hb b'' 0) + pow2 8 * v (get hb b'' 1)+ pow2 16 * v (get hb b'' 2)+ pow2 24 * v (get hb b'' 3))
+    /\ v b12 = U8.(v (get hb b''' 0) + pow2 8 * v (get hb b''' 1)+ pow2 16 * v (get hb b''' 2)+ pow2 24 * v (get hb b''' 3))))
     (ensures (lemma_add_word_post a0 a4 a8 a12 b0 b4 b8 b12 ha a hb b))
 let lemma_add_word ha a hb b a0 a4 a8 a12 b0 b4 b8 b12 =
   lemma_add_word_1 ha a a0 a4 a8 a12; lemma_add_word_1 hb b b0 b4 b8 b12;
@@ -1401,7 +1401,7 @@ val lemma_add_word2_2:
       /\ U8.v (get h b3 1) = (U32.v z3 / pow2 8) % pow2 8
       /\ U8.v (get h b3 2) = (U32.v z3 / pow2 16) % pow2 8
       /\ U8.v (get h b3 3) = (U32.v z3 / pow2 24)  % pow2 8 ))
-    (ensures (little_endian (as_seq h b) = U32 (v z0 + pow2 32 * v z1 + pow2 64 * v z2 + pow2 96 * v z3)))
+    (ensures (little_endian (as_seq h b) = U32.(v z0 + pow2 32 * v z1 + pow2 64 * v z2 + pow2 96 * v z3)))
 let lemma_add_word2_2 ha a z0 z1 z2 z3 =
   lemma_as_seq_sub ha a 0ul  4ul;
   lemma_as_seq_sub ha a 4ul  4ul;
@@ -1463,7 +1463,7 @@ val lemma_add_word2:
       /\ U8.v (get h4 b3 1) = (U32.v z3 / pow2 8) % pow2 8
       /\ U8.v (get h4 b3 2) = (U32.v z3 / pow2 16) % pow2 8
       /\ U8.v (get h4 b3 3) = (U32.v z3 / pow2 24)  % pow2 8 ))
-    (ensures (little_endian (as_seq h4 b) = U32 (v z0 + pow2 32 * v z1 + pow2 64 * v z2 + pow2 96 * v z3)))
+    (ensures (little_endian (as_seq h4 b) = U32.(v z0 + pow2 32 * v z1 + pow2 64 * v z2 + pow2 96 * v z3)))
 let lemma_add_word2 h0 h1 h2 h3 h4 b z0 z1 z2 z3 =
   lemma_add_word2_1 h0 h1 h2 h3 h4 b z0 z1 z2 z3;
   lemma_add_word2_2 h4 b z0 z1 z2 z3
