examples/low-level/crypto/Crypto.Symmetric.Poly1305.Spec.fst
@@ -127,7 +127,7 @@ let rec eq_poly_spec p0 p1 r =
 
 
 private val fix: word_16 -> i:nat{i < 16} -> m:U8.t -> Tot word_16
-let fix r i m = Seq.upd r i (U8 (Seq.index r i &^ m))
+let fix r i m = Seq.upd r i (U8.(Seq.index r i &^ m))
 
 (** Abstract spec of clamping for the state invariant.
     For our polynomial-sampling assumption, we rely solely on the number of
