examples/low-level/crypto/Crypto.Symmetric.UF1CMA.fst
@@ -56,7 +56,7 @@ type skey (rgn:rid) (i:id) =
 //16-10-16 can't make it abstract?
 (** Conditionally-allocated abstract key (accessed only in this module) *)
 let akey (rgn:rid) (i:id) = 
-  o:option (skey rgn i) {is_Some o <==> skeyed i}
+  o:option (skey rgn i) {Some? o <==> skeyed i}
   // using a sum type for KreMLin. Was: if skeyed i then skey rgn i else unit
 
 val get_skey: #r:rid -> #i:id{skeyed i} -> akey r i -> Tot (skey r i)
@@ -381,7 +381,7 @@ val verify:
     disjoint_2 (MAC.as_buffer st.r) st.s tag /\
     acc_inv st acc h0 /\
     (mac_log ==> RR.m_contains (ilog st.log) h0) /\
-    (mac_log /\ authId i ==> is_Some (RR.m_sel h0 (ilog st.log)))))
+    (mac_log /\ authId i ==> Some? (RR.m_sel h0 (ilog st.log)))))
   (ensures (fun h0 b h1 ->
     Buffer.modifies_0 h0 h1 /\
     live h0 st.s /\ 
